Finish IntOrBool

pulse/examples/steel/arraystructs/IntOrBool.fst
@@ -1,12 +1,14 @@
 module IntOrBool
 
-open AggregateRef
+#push-options "--print_universes"
+
 open FStar.PCM
-open FStar.PCM.Extras
 open FStar.PCM.POD
+open Steel.C.PCM
 open Steel.Effect
 module M = Steel.Memory
 module A = Steel.Effect.Atomic
+module U = FStar.Universe
 
 let int_or_bool_cases k = match k with
   | I -> pod int
@@ -15,67 +17,90 @@ let int_or_bool_cases k = match k with
 let int_or_bool_cases_pcm k: pcm (int_or_bool_cases k) = match k with
   | I -> pod_pcm int
   | B -> pod_pcm bool
-let int_or_bool = union int_or_bool_cases_pcm
+  
+let int_or_bool = union #int_or_bool_case #int_or_bool_cases int_or_bool_cases_pcm
+
 let int_or_bool_pcm: pcm int_or_bool = union_pcm int_or_bool_cases_pcm
 
-let mk_int i = Some (|I, Ghost.reveal i|)
-let mk_bool b = Some (|B, Ghost.reveal b|)
+let mk_int i = Ghost.hide (field_to_union_f int_or_bool_cases_pcm I (Ghost.reveal i))
+let mk_bool b = Ghost.hide (field_to_union_f int_or_bool_cases_pcm B (Ghost.reveal b))
 
-let re_i = case_refinement int_or_bool_cases_pcm I
-let re_b = case_refinement int_or_bool_cases_pcm B
+let _i = union_field int_or_bool_cases_pcm I
+let _b = union_field int_or_bool_cases_pcm B
 
-/// Lenses for cases
+open FStar.FunctionalExtensionality
 
-let _i = case int_or_bool_cases_pcm I
-let _b = case int_or_bool_cases_pcm B
+let case_of_int_or_bool u =
+  let k = case_of_union int_or_bool_cases_pcm u in
+  match k with
+  | Some I ->
+    assert (~ (Ghost.reveal u I == one (pod_pcm int)));
+    assert (exists (x:int). (Ghost.reveal u I == Ghost.reveal (some (Ghost.hide x))));
+    assert (exists (x:int). (Ghost.reveal u I == Ghost.reveal (some (Ghost.hide x))) /\ u `feq` mk_int (Ghost.hide (Ghost.reveal (some (Ghost.hide x)))));
+    assert (exists i. u == mk_int i); k
+  | Some B -> 
+    assert (~ (Ghost.reveal u B == one (pod_pcm bool)));
+    assert (exists (b:bool). Ghost.reveal u B == Ghost.reveal (some (Ghost.hide b)) /\ u `feq` mk_bool (Ghost.hide (Ghost.reveal (some (Ghost.hide b))))); k
+  | None -> None
+  
+let case_of_int_or_bool_int _ = ()
+let case_of_int_or_bool_bool _ = ()
+let case_of_int_or_bool_one = ()
 
-/// Taking pointers to the i and b cases of an int_or_bool
+let mk_int_exclusive i = exclusive_union_intro int_or_bool_cases_pcm (mk_int i) I
 
-let addr_of_i (#i: Ghost.erased (pod int)) (p: ref 'a int_or_bool_pcm)
-: SteelT (q:ref 'a (pod_pcm int){q == ref_focus (ref_refine p re_i) _i})
+let mk_bool_exclusive b = exclusive_union_intro int_or_bool_cases_pcm (mk_bool b) B
+
+let addr_of_i (#i: Ghost.erased (nonunit (pod_pcm int))) (p: ref 'a int_or_bool_pcm)
+: SteelT (q:ref 'a (pod_pcm int){q == ref_focus p _i})
     (p `pts_to` mk_int i)
-    (fun q -> q `pts_to` i)
-= let mk_int_i : Ghost.erased (refine_t (refinement_f re_i)) = Some (|I, Ghost.reveal i|) in
-  A.change_equal_slprop (p `pts_to` mk_int i) (p `pts_to` Ghost.reveal mk_int_i);
-  addr_of_union_lens p _i (Ghost.reveal mk_int_i)
+    (fun q -> q `pts_to` Ghost.reveal i)
+= let q = addr_of_union_field p I (mk_int i) in
+  A.change_equal_slprop (q `pts_to` _) (q `pts_to` _);
+  A.return q
 
-let unaddr_of_i (#i: Ghost.erased (pod int)) (#opened: M.inames)
+let unaddr_of_i (#i: Ghost.erased (nonunit (pod_pcm int))) (#opened: M.inames)
   (p: ref 'a int_or_bool_pcm)
-  (q: ref 'a (pod_pcm int){q == ref_focus (ref_refine p re_i) _i})
-: A.SteelGhostT unit opened (q `pts_to` i) (fun _ -> p `pts_to` mk_int i)
-= unaddr_of_union_lens q p _i i
+  (q: ref 'a (pod_pcm int){q == ref_focus p _i})
+: A.SteelGhostT unit opened (q `pts_to` Ghost.reveal i) (fun _ -> p `pts_to` mk_int i)
+= unaddr_of_union_field I q p (Ghost.reveal i);
+  A.change_equal_slprop (p `pts_to` _) (p `pts_to` _)
 
-let addr_of_b (#b: Ghost.erased (pod bool)) (p: ref 'a int_or_bool_pcm)
-: SteelT (q:ref 'a (pod_pcm bool){q == ref_focus (ref_refine p re_b) _b})
+let addr_of_b (#b: Ghost.erased (nonunit (pod_pcm bool))) (p: ref 'a int_or_bool_pcm)
+: SteelT (q:ref 'a (pod_pcm bool){q == ref_focus p _b})
     (p `pts_to` mk_bool b)
-    (fun q -> q `pts_to` b)
-= let mk_bool_b : Ghost.erased (refine_t (refinement_f re_b)) = Some (|B, Ghost.reveal b|) in
-  A.change_equal_slprop (p `pts_to` mk_bool b) (p `pts_to` Ghost.reveal mk_bool_b);
-  addr_of_union_lens p _b (Ghost.reveal mk_bool_b)
+    (fun q -> q `pts_to` Ghost.reveal b)
+= let q = addr_of_union_field p B (mk_bool b) in
+  A.change_equal_slprop (q `pts_to` _) (q `pts_to` _);
+  A.return q
 
-let unaddr_of_b (#b: Ghost.erased (pod bool)) (#opened: M.inames)
+let unaddr_of_b (#b: Ghost.erased (nonunit (pod_pcm bool))) (#opened: M.inames)
   (p: ref 'a int_or_bool_pcm)
-  (q: ref 'a (pod_pcm bool){q == ref_focus (ref_refine p re_b) _b})
-: A.SteelGhostT unit opened (q `pts_to` b) (fun _ -> p `pts_to` mk_bool b)
-= unaddr_of_union_lens q p _b b
-
-/// Switching the case
-
-let switch_to_bool (#i: Ghost.erased int)
-  (p: ref 'a int_or_bool_pcm) (b: bool)
-: SteelT unit (p `pts_to` mk_int (some i)) (fun _ -> p `pts_to` mk_bool (some b))
-= let u: int_or_bool = Some (|B, Some b|) in
-  assume (forall frame.
-    composable int_or_bool_pcm (mk_int (some i)) frame ==> 
-    composable int_or_bool_pcm u frame);
-  assert (valid_write int_or_bool_pcm (mk_int (some i)) u);
-  ref_write p u;
+  (q: ref 'a (pod_pcm bool){q == ref_focus p _b})
+: A.SteelGhostT unit opened (q `pts_to` Ghost.reveal b) (fun _ -> p `pts_to` mk_bool b)
+= unaddr_of_union_field B q p (Ghost.reveal b);
   A.change_equal_slprop (p `pts_to` _) (p `pts_to` _)
 
-let switch_to_int (#b: Ghost.erased bool)
+let switch_to_int_fpu (#u: Ghost.erased int_or_bool{exclusive int_or_bool_pcm (Ghost.reveal u)})
   (p: ref 'a int_or_bool_pcm) (i: int)
-: SteelT unit (p `pts_to` mk_bool (some b)) (fun _ -> p `pts_to` mk_int (some i))
-= let u: int_or_bool = Some (|I, Some i|) in
-  assume (valid_write int_or_bool_pcm (mk_bool (some b)) u);
-  ref_write p u;
-  A.change_equal_slprop (p `pts_to` _) (p `pts_to` _)
+: frame_preserving_upd int_or_bool_pcm u (mk_int (Ghost.hide (Ghost.reveal (some (Ghost.hide i)))))
+= base_fpu int_or_bool_pcm u (field_to_union_f int_or_bool_cases_pcm I (Some i))
+
+let switch_to_int (#u: Ghost.erased int_or_bool)
+  (p: ref 'a int_or_bool_pcm) (i: int)
+: Steel unit
+    (p `pts_to` u)
+    (fun _ -> p `pts_to` mk_int (Ghost.hide (Ghost.reveal (some i))))
+    (requires fun _ -> Some? (case_of_int_or_bool u) /\ exclusive int_or_bool_pcm u)
+    (ensures fun _ _ _ -> True)
+= ref_upd p _ _ (switch_to_int_fpu p i)
+
+let switch_to_bool (#u: Ghost.erased int_or_bool)
+  (p: ref 'a int_or_bool_pcm) (b: bool)
+: Steel unit
+    (p `pts_to` u)
+    (fun _ -> p `pts_to` mk_bool (Ghost.hide (Ghost.reveal (some b))))
+    (requires fun _ -> Some? (case_of_int_or_bool u) /\ exclusive int_or_bool_pcm u)
+    (ensures fun _ _ _ -> True)
+= ref_upd p u (mk_bool (Ghost.hide (Ghost.reveal (some (Ghost.hide b)))))
+    (base_fpu int_or_bool_pcm u (field_to_union_f int_or_bool_cases_pcm B (Some b)))
